theories/typing_inversion.v
@@ -169,6 +169,18 @@ Definition be_principal_typing (C: t_context) (be: basic_instruction) (tf: instr
         lookup_N (tc_tables C) x = Some tabt /\
         tabt.(tt_elem_type) = T_funcref /\
         lookup_N (tc_types C) y = Some (Tf ts1 ts2)
+  | BI_return_call n =>
+      exists ts1 ts2 ts3 ts4,
+      tf = (Tf (ts3 ++ ts1) ts4) /\
+        lookup_N (tc_funcs C) n = Some (Tf ts1 ts2) /\
+        tc_return C = Some ts2
+  | BI_return_call_indirect x y =>
+      exists ts1 ts2 ts3 ts4 tabt,
+      tf = (Tf (ts3 ++ ts1 ++ [::T_num T_i32]) ts4)/\
+        lookup_N (tc_tables C) x = Some tabt /\
+        tabt.(tt_elem_type) = T_funcref /\
+        lookup_N (tc_types C) y = Some (Tf ts1 ts2) /\
+        tc_return C = Some ts2
   | BI_local_get x =>
       exists t,
       tf = (Tf nil [::t]) /\
@@ -522,6 +534,10 @@ Definition e_principal_typing (s: store_record) (C: t_context) (e: administrativ
   | AI_invoke a =>
       exists tf0, tf = tf0 /\
         ext_func_typing s a = Some tf0
+  | AI_return_invoke a =>
+      exists ts1 ts2 ts3 ts4, tf = (Tf (ts3 ++ ts1) ts4) /\
+      ext_func_typing s a = Some (Tf ts1 ts2) /\
+      tc_return C = Some ts2                     
   | AI_label n es0 es =>
       exists ts1 ts2,
       tf = (Tf nil ts2) /\
@@ -564,7 +580,7 @@ Lemma e_typing_inversion: forall s C e tf,
       e_principal_typing s C e tf_principal.
 Proof.
   move => s C e tf HType.
-  dependent induction HType; try by (eexists; split; first (by apply instr_subtyping_eq); try by eexists; eauto).
+  dependent induction HType; try by (eexists; split; first (by apply instr_subtyping_eq); try by repeat (eexists; eauto)).
   (* bet *)
   - do 2 (try destruct bes => //).
     destruct e => //.
